cleaned it up

Caches/StoreAtomicity.v
@@ -1,24 +1,28 @@
-Require Import DataTypes.
+Require Import DataTypes Transitions.
 
 Set Implicit Arguments.
 
 Section StoreAtomicity.
-  Variable getStreamIo: Time -> option (Addr * Cache * Data * Desc * Data).
+  Variable State: Set.
+  Variable Trans: AllTransitions State.
+  Variable initState: State.
+  Variable stm: Stream Trans initState.
+  Variable getTransIo: forall s s', Trans s s' -> option (Addr * Cache * Data * Desc * Data). 
 
   Record StoreAtomicity := {
    storeAtomicityLd:
     forall a c d ld t,
-      getStreamIo t = Some (a, c, d, Ld, ld) ->
+      getStreamIo getTransIo t stm = Some (a, c, d, Ld, ld) ->
       (d = initData zero /\ ld = initData a /\
      forall {ti}, 0 <= ti < t -> forall ci di ldi, defined ci ->
-                                   ~ getStreamIo ti = Some (a, ci, di, St, ldi)) \/
-    (exists cb tb ldb, defined cb /\ tb < t /\ getStreamIo tb = Some (a, cb, ld, St, ldb) /\
+                                   ~ getStreamIo getTransIo ti stm = Some (a, ci, di, St, ldi)) \/
+    (exists cb tb ldb, defined cb /\ tb < t /\ getStreamIo getTransIo tb stm = Some (a, cb, ld, St, ldb) /\
       forall ti, tb < ti < t ->
                    forall ci di ldi, defined ci ->
-                     ~ getStreamIo ti = Some (a, ci, di, St, ldi));
+                     ~ getStreamIo getTransIo ti stm = Some (a, ci, di, St, ldi));
 
    storeAtomicitySt:
    forall a c d ld t,
-     getStreamIo t = Some (a, c, d, St, ld) ->
+     getStreamIo getTransIo t stm = Some (a, c, d, St, ld) ->
      ld = initData zero}.
 End StoreAtomicity.
