Caches/Top.v
@@ -1,5 +1,5 @@
 Require Import DataTypes L1 StoreAtomicity LatestValue Cache Channel Compatible
-Rules ChannelAxiom L1Axioms CompatBehavior LatestValueAxioms BehaviorAxioms MsiState.
+Rules ChannelAxiom L1Axioms CompatBehavior LatestValueAxioms BehaviorAxioms MsiState Transitions.
 
 Set Implicit Arguments.
   Module l1 := mkL1Axioms.
@@ -52,4 +52,70 @@ Set Implicit Arguments.
     assumption.
   Qed.
 
-  Definition cacheIsStoreAtomic := Build_StoreAtomicity getStreamCacheIo storeAtomicityLd' storeAtomicitySt'.
+  Theorem sameThing t:
+    getStreamCacheIo t = getCacheIo _ _ (getStreamTransition t cstm).
+  Proof.
+    admit.
+  Qed.
+
+  Theorem cacheIsStoreAtomic : StoreAtomicity cstm getCacheIo.
+  Proof.
+    assert  (forall (a : Addr) (c : Tree) (d ld : Data) (t : Time),
+      getCacheIo _ _ (getStreamTransition t cstm) = Some (a, c, d, Ld, ld) ->
+      d = initData zero /\
+      ld = initData a /\
+      (forall ti : nat,
+       0 <= ti < t ->
+       forall (ci : Tree) (di ldi : Data),
+       defined ci -> getCacheIo _ _ (getStreamTransition ti cstm) <> Some (a, ci, di, St, ldi)) \/
+      (exists (cb : Tree) (tb : nat) (ldb : Data),
+         defined cb /\
+         tb < t /\
+         getCacheIo _ _ (getStreamTransition tb cstm) = Some (a, cb, ld, St, ldb) /\
+         (forall ti : nat,
+          tb < ti < t ->
+          forall (ci : Tree) (di ldi : Data),
+          defined ci -> getCacheIo _ _ (getStreamTransition ti cstm) <> Some (a, ci, di, St, ldi)))).
+    intros.
+    pose proof (@storeAtomicityLd' a c d ld t).
+    destruct H0.
+    pose proof (sameThing t).
+    rewrite H in H0.
+    assumption.
+    left.
+    constructor; intuition.
+    specialize (H3 ti (conj H4 H5) ci di ldi H2).
+    pose proof (sameThing ti).
+    rewrite <- H7 in H6.
+    intuition.
+    right.
+    destruct H0 as [cb [tb [ldb [defcb [cond [sth  rest]]]]]].
+    exists cb, tb, ldb.
+    constructor.
+    intuition.
+    constructor.
+    intuition.
+    constructor.
+    pose proof (sameThing tb).
+    rewrite H0 in sth.
+    assumption.
+    intros.
+    specialize (rest ti H0 ci di ldi H1).
+    pose proof (sameThing ti).
+    rewrite H2 in rest.
+    assumption.
+    
+
+    assert (great: forall a c d ld t,
+      getCacheIo _ _ (getStreamTransition t cstm) = Some (a, c, d, St, ld) ->
+      ld = initData zero).
+
+    intros.
+
+    pose proof (sameThing t).
+    rewrite <- H1 in H0.
+    pose proof (@storeAtomicitySt' a c d ld t H0).
+    intuition.
+
+    apply (Build_StoreAtomicity _ _ H great).
+  Qed.
